---
title: "Proof: properties of sigma notation"
author: "Tom Coleman"
abstract-title: Summary
abstract: An explanation as to why some of the properties of sigma notation are true.
draft: true

---

*Before reading this proof sheet, it is recommended that you read [Guide: Introduction to sigma notation](../studyguides/sigmanotation.qmd) and [Guide: Proof by induction].*

# Proof of properties of sigma notation {-}

## Distributivity

::: {.callout-note}

## Distributivity

Hello

:::

::: {.callout-note}

## Proof of distributivity

You can see this is true by writing the entire sum out, like this:

$$
\begin{array}{rcl}
\sum_{i=k}^nCa_i &=& Ca_k + Ca_{k+1} + Ca_{k+2} + \ldots + Ca_n \\
&=& C(a_k + a_{k+1} + a_{k+2} + \ldots + a_n) \\
&=& C\sum_{i=k}^n a_k
\end{array}
$$

:::

## Combining and decomposing sums

::: {.callout-note}

## Combining and decomposing sums

Hello

:::

::: {.callout-note}

## Proof of combining and decomposing sums

Similar to the distributive property, you can show this is true by writing the entire sum out: 

$$
\begin{array}{rcl} 
\sum_{i=k}^na_i + \sum_{i=k}^n b_i &=& (a_{k} + a_{k+1} + \ldots + a_n) + (b_k + b_{k+1} + \ldots + b_n) \\ & = & (a_k + b_k) + (a_{k+1} + b_{k+1}) + \ldots + (a_n + b_n) \\[0.5em] & = & \sum_{i=k}^n (a_k + b_k).
\end{array}
$$

In a similar way, you can show that $\sum_{i=k}^n a_i - \sum_{i=k}^n b_i = \sum_{i=k}^n(a_i-b_i)$ is also true.

:::

# Further reading {-}

[Guide: Using the quadratic formula](../studyguides/quadraticformula.qmd)

[Questions: Using the quadratic formula](../questions/qs-quadraticformula.qmd)

## Version history {-}

v1.0: created in 04/24 by tdhc. 

