---
title: "Answers: Introduction to rearranging equations"
author: "Shanelle Advani, Tom Coleman"
abstract-title: Summary
abstract: Answers to questions relating to the guide on introduction to rearranging equations.

---

*These are the answers to [Questions: Introduction to rearranging equations](../questions/qs-introtorearrange.qmd).* 

**Please attempt the questions before reading these answers!**


## Q1 {-}

1.1. $\quad a = x - 2b$

1.2. $\quad b = \dfrac{x-a}{2}$

1.3. $\quad z = - \dfrac{x}{4} + \dfrac{y}{2} + 1$

1.4. $\quad x = \dfrac{3y}{5} - \dfrac{8z}{5} -\dfrac{2}{5}$

1.5. $\quad y = \dfrac{5x}{3} +\dfrac{8z}{3} + \dfrac{2}{3}$

1.6. $\quad z = -\dfrac{5x}{8} + \dfrac{3y}{8} - \dfrac{1}{4}$

1.7. $\quad x = \pm\sqrt{4-y^2}$

1.8. $\quad x = \pm\sqrt{4a - \dfrac{y^2}{4}}$

1.9. $\quad y = \pm\sqrt{16a - 4x^2}$

1.10. $\quad x = \pm\sqrt{(y+1)^2 + a^2}$

1.11. $\quad a = \sqrt[3]{x^3 - (y+1)^3}$

1.12. $\quad x = \sqrt[3]{(y+1)^3 - a^3}$

1.13. $\quad d = \dfrac{a^3 - x^4y^2}{2bc}$

1.14. $\quad a = \sqrt[3]{x^4y^2 - 2bcd}$

1.15. $\quad x = \pm\sqrt[4]{\dfrac{a^3 + 2bcd}{y^2}}$

1.16. $\quad x = \dfrac{1}{ly^2 - 45}$

## Q2 {-}

$\quad a = \dfrac{5x^3y^3}{4bc^2} + \dfrac{6z}{4bc^2w^4}$

 

$\quad b = \dfrac{5x^3y^3}{4ac^2} + \dfrac{6z}{4ac^2w^4}$

 

$\quad c = \pm\sqrt{\dfrac{5x^3y^3}{4ab} + \dfrac{6z}{4abw^4}}$

 

$\quad y = \sqrt[3]{\dfrac{4abc^2}{5x^3} - \dfrac{6z}{5w^4x^3}}$

 

$\quad z = \dfrac{4abc^2w^4 - 5w^4x^3y^3}{6}$

 

$\quad w = \sqrt[4]{\dfrac{6z}{4abc^2 - 5x^3y^3}}$

---

---
