---
title: "Answers: Logarithms"
author: "Zoe Gemmell"
abstract-title: Summary
abstract: Answers to questions relating to the study guide on logarithms.

---

*These are answers to: [Questions: Logarithms](../questions/qs-logarithms.qmd).* 

**Please attempt the questions before reading these answers!**

Throughout this answer sheet, the natural logarithm $\log_e(x)$ is written as $\ln(x)$.

---

## Q1 {-}

1.1. $\quad \log_{7}(x) = 1$ rearranged gives $7^1=x$ so $x=7$.
 

1.2. $\quad \log_{8}(x) = 3$ rearranged gives $8^3=x$ so $x=512$.
 

1.3. $\quad \log_{12}(x) = 0$ rearranged gives $12^0=x$ so $x=1$.
 

1.4. $\quad \log_{10}(100) = x$ rearranged gives $10^x=100$ so $x=2$.
 

1.5. $\quad \log_{2}(64) = x$ rearranged gives $2^x=64$ so $x=6$.
 

1.6. $\quad \log_{4}(2) = x$ rearranged gives $4^x=2$ so $x=\dfrac{1}{2}$.
 

1.7. $\quad \log_{3}(27) = x$ rearranged gives $3^x=27$ so $x=3$.
 

1.8. $\quad \log_{10}(1) = x$ rearranged gives $10^x=1$ so $x=0$.
 

1.9. $\quad \log_{x}(16) = 4$ rearranged gives $x^4=16$ so $x=\sqrt[4]{16}=2$.
 

1.10. $\quad \log_{x}(49) = 2$ rearranged gives $x^2=49$ so $x=\sqrt{49}=7$.
 

1.11. $\quad \log_{x}(13) = 4$ rearranged gives $x^4=13$ so $x=\sqrt[4]{13}$.
 

1.12. $\quad \log_{2x}(12) = -1$ rearranged gives $(2x)^{-1}=12$ so $x=\dfrac{1}{24}$.

## Q2 {-}

The product rule: $\log_{a}(M\cdot N)=\log_{a}(M)+\log_{a}(N)$

The quotient rule: $\log_{a}\left(\dfrac{M}{N}\right)=\log_{a}(M)-\log_{a}(N)$

The power rule: $\log_{a}(M^k)=k\cdot\log_{a}(M)$

The zero rule: $\log_{a}(1)=0$

The identity rule: $\log_{a}(a)=1$

2.1. The solution to $\log_{3}(\dfrac{1}{27}) = x$ is $x = -1/3$.
 

<!-- \begin{align*} -->
<!-- x&=\log_{3}(1)-\log_{3}(27)\tag{\,Using Law 2} \\[0.5em] -->
<!-- &=0-\log_{3}(27)\tag{\,Using Law 4}\\[0.5em] -->
<!-- -x&=\log_{3}(27) -->
<!-- \end{align*} -->
<!-- Let $y=-x$, so Rearranging gives: $3^y=27$, so $y=3=-x$ implying that $x=-3$\ -->

2.2. The solution to $4\log_{4}(2) = x$ is $x = 2$. 
 

<!-- \begin{align*} -->
<!-- x&=\log_{4}(4^2)\nonumber \\[0.5em] -->
<!-- &=2\cdot \log_{4}(4)\tag{\,Using Law 3} \\[0.5em] -->
<!-- &=2\cdot 1 \tag{\,Using Law 5} \\[0.5em] -->
<!-- &=2 -->
<!-- \end{align*} -->

2.3. The solution to $\log_{5}(10) + \log_{5}\left(\dfrac{5}{2}\right)=x$ is $x = 2$.
 

2.4. The solution to $3\log_{7}\left(a^{1/3}\right) - \frac{1}{2}\log_{7}(a^2) = x$ is $x = 0$. 
 

<!-- \begin{align*} -->
<!-- x&=\log_{7}(2)-\log_{7}(49)\tag{\,Using Law 2} \\[0.5em] -->
<!-- &=\log_{7}(2)-2\nonumber \\[0.5em] -->
<!-- x+2&=\log_{3}(27) -->
<!-- \end{align*} -->
<!-- Rearranging gives: $3^{x+2}=27$, so $x+2=3$ implying that $x=1$\ -->

2.5. The solution to $\log_{x}(YZ) = M$ is $x=\sqrt[M]{YZ}$.
 

2.6. The solution to $\log_{a}\left(y\right) - \log_a(x) = 11$ is $x = ya^{-11}$.
 

<!-- \begin{align*} -->
<!-- 1&=\log_{6}(36)-\log_{6}(x)\tag{\,Using Law 2} \\[0.5em] -->
<!-- &=2-\log_{6}(x)\nonumber \\[0.5em] -->
<!-- \log_{6}(x)&=1\nonumber \\[0.5em] -->
<!-- 6^1&=x -->
<!-- \end{align*} -->

<!-- 2.6. $\log_{5}(25)=x$\ -->
<!-- \begin{align*} -->
<!-- x&=\log_{5}(5\cdot5)\tag{\,Using Law 1} \\[0.5em] -->
<!-- &=\log_{5}(5)+\log_{5}(5)\nonumber \\[0.5em] -->
<!-- &=1+1 \tag{\,Using Law 5} \\[0.5em] -->
<!-- &=2 -->
<!-- \end{align*} -->

## Q3 {-}

3.1. $\log_3(25)$ is equal to $\dfrac{2}{\log_5(3)}$.
 

<!-- \begin{align*} -->
<!-- \log_3(25)=\dfrac{\log_5(25)}{\log_5(3)}\end{align*} -->

3.2. $\log_{8}(3)$ is equal to $\dfrac{4\log_{16}(3)}{3}$. 
 
<!-- \begin{align*} -->
<!-- \log_{4}(64)=\dfrac{\log_{16}(64)}{\log_{16}(4)}\end{align*} -->

3.3. $\log_{e}(10)$ is equal to $\dfrac{1}{\log_{1000}(e^3)}$.
 
<!-- \begin{align*} -->
<!-- \log_{e}(100)=\dfrac{2}{\log_{10}(e)}\end{align*} -->

3.4. $\ln(27)$ is equal to $\dfrac{3}{\log_{3}(e)}$.
 

<!-- \begin{align*} -->
<!-- \ln(27)=\log_{3}(27)\end{align*} -->

3.5. $\log_{4}(8x)$ is equal to $\dfrac{3}{2} + \log_2\left(\sqrt{2}\right)$.
 

<!-- \begin{align*} -->
<!-- \log_{4}(8)=\dfrac{\log_{2}(8)}{\log_{2}(4)}=\dfrac{3}{2}\end{align*} -->


---